ctx-equiv-ixfree/context_tests.v
@@ -1,0 +1,56 @@
+
+From CtxEquivIxFree Require Import lang.
+
+(*
+
+Inside-out and outside-in contexts
+
+Assuming 2 is the innermost application, ((1 2) 3),
+and we are trying to plug 1 into its place in this expression,
+
+The syntax of contexts is the same, but their structure is .
+
+E ::= □ | E e | v E
+
+standard outside-in contexts:
+
+  □[□ 3][□ 2]
+= (□ 3)[□ 2]
+= ((□ 2) 3)
+
+rplug ((□ 2) 3) 1
+= ((rplug (□ 2) 1) 3)
+= (((rplug □ 1) 2) 3)
+= ((1 2) 3)
+
+inside-out contexts:
+hole args are the surrounding context,
+and the topmost term is the innermost context.
+
+plug ((□ 3) 2) 1
+= plug (□ 3) (1 2)
+= plug □ ((1 2) 3)
+= ((1 2) 3)
+
+https://www.williamjbowman.com/teaching/2020/w1/cpsc509/resources/05-reduction.pdf
+
+*)
+
+(* for one level of nesting, both kinds of contexts behave the same *)
+Example ex_plug1:
+  plug ectx_hole (vint 1) = rplug rctx_hole (vint 1).
+Proof. reflexivity. Qed.
+
+Example ex_plug2:
+    plug (ectx_app1 ectx_hole (vint 2)) (vint 1)
+  = rplug (rctx_app1 rctx_hole (vint 2)) (vint 1).
+Proof. reflexivity. Qed.
+
+(* this is where they start to differ *)
+Example ex_plug3: plug (ectx_app1 (ectx_app1 ectx_hole (vint 3)) (vint 2))
+  (ret (vint 1)) = app (app (vint 1) (vint 2)) (vint 3).
+Proof. reflexivity. Qed.
+
+Example ex_rplug3: rplug (rctx_app1 (rctx_app1 rctx_hole (vint 3)) (vint 2))
+  (ret (vint 1)) = app (app (vint 1) (vint 3)) (vint 2).
+Proof. reflexivity. Qed.
